Work in progress.

src/coq/optimisations/SANDBOX/FindSearch.v
@@ -1,3 +1,5 @@
+Require Import EqNat.
+
 (* Consider the following structure: *)
 
 Definition iid := nat.
@@ -7,11 +9,25 @@ Definition bid := nat.
 Definition fid := nat.
 
 Definition listA := list (bid * data).
-Definition listB := list (fid * listA).
 
 
-Fixpoint searchListA (b:bid) (l:listA) : option (bid * data) :=
+Fixpoint find (b:bid) (l:listA) : option data :=
 match l with
   | nil => None
-  | (_::_)%list => None
+  | ((fst, snd) :: tl)%list => if beq_nat fst b then Some snd else find b tl
 end.
+
+
+
+Definition two_fold (b:bid) (l l1:listA) : option data :=
+match (find b l) with
+  | None => match (find b l1) with
+           | None => None
+           | Some a => Some a
+            end
+  | Some a => Some a
+end.
+
+
+
+Lemma two_consecutive_eq 
